prove inv is preserved by add_liquidity

AMM.thy
@@ -1,5 +1,5 @@
 theory AMM
-  imports "Word_Lib.Machine_Word_64" HOL.Real
+  imports (*"Word_Lib.Machine_Word_64"*) HOL.Real
 begin
 
 section "Pool state"
@@ -14,55 +14,62 @@ definition k where "k p \<equiv> (x p)*(y p)"
 section "Adding liquidity"
 
 definition add_liquidity_spec where
-  "add_liquidity_spec p \<Delta>x \<equiv> let \<alpha> = \<Delta>x / (x p)
-    in \<lparr>x = ((1+\<alpha>)*(x p)), y = ((1+\<alpha>)*(y p)), l = ((1+\<alpha>)*(l p))\<rparr>"
+  "add_liquidity_spec p \<Delta>x \<equiv> let \<alpha> = \<Delta>x / x p
+    in \<lparr>x = (1+\<alpha>)*(x p), y = (1+\<alpha>)*(y p), l = (1+\<alpha>)*(l p)\<rparr>"
 
-definition add_liquidity_code where
-  "add_liquidity_code p \<Delta>x \<equiv>
-    \<lparr>x = ((x p) + \<Delta>x),
-     y = ((y p) + \<lfloor>(\<Delta>x*(y p)) / (x p)\<rfloor> + 1),
-     l = ((l p) + \<lfloor>(\<Delta>x*(l p)) / (x p)\<rfloor>)\<rparr>"
+definition add_liquidity_code_spec where
+  "add_liquidity_code_spec p \<Delta>x \<equiv>
+    \<lparr>x = x p + \<Delta>x,
+     y = y p + \<lfloor>\<Delta>x*(y p) / x p\<rfloor> + 1, \<comment> \<open>note we need to round in favor of the pool here\<close>
+     l = l p + \<lfloor>\<Delta>x*(l p) / x p\<rfloor>\<rparr>"
 
-lemma thm_1:
+lemma l1:"(1 + \<Delta>x / x p) * a = a + \<Delta>x * a / x p" for a
+  \<comment> \<open>this simple lemma helps automated provers a lot\<close>
+  by algebra
+
+lemma add_liquidity_properties:  
   \<comment> \<open>properties of add_liquidity\<close>
   fixes p \<Delta>x
   assumes "x p > 0" and "y p > 0" and "l p > 0"
     and "\<Delta>x > 0"
   defines "p' \<equiv> add_liquidity_spec p \<Delta>x"
-    and "p'' \<equiv> add_liquidity_code p \<Delta>x"
-  shows "x p < x p'" and "x p' = x p''" and "y p < y p'"
-    and "y p' < y p''" and "y p'' \<le> y p' + 1"
-    and "l p' - 1 < l p''" and "l p'' \<le> l p'"
+    and "p'' \<equiv> add_liquidity_code_spec p \<Delta>x"
+  shows "x p < x p'" and "x p' = x p''"
+    and "y p < y p'" and "y p' < y p''" and "y p'' \<le> y p' + 1"
+    and "l p' - 1 < l p''" and "l p'' \<le> l p'" and "l p \<le> l p''" and "l p < l p'"
     and "k p < k p'" and "k p' < k p''"
-    and "(k p')/(k p) = ((l p')/(l p))\<^sup>2"
-    and "((l p'')/(l p))\<^sup>2 < (k p'')/(k p)"
+    and "k p'/k p = (l p'/l p)\<^sup>2"
+    and "(l p''/l p)\<^sup>2 < k p''/k p"
+    and "x p / l p = x p' / l p'"
+    and "y p / l p = y p' / l p'"
 proof -
-  have l1:"(1 + \<Delta>x / x p) * a = a + \<Delta>x * a / x p" for a
-    \<comment> \<open>this simple lemma helps automated provers a lot\<close>
-    by algebra
   show "x p < x p'"
     by (metis add.commute add_liquidity_spec_def assms(1,4) div_self l1 less_add_same_cancel2 mult.comm_neutral order_less_irrefl p'_def select_convs(1) times_divide_eq_right)
   show "x p' = x p''"
-    using assms(1-4) unfolding p'_def p''_def add_liquidity_spec_def add_liquidity_code_def Let_def
+    using assms(1-4) unfolding p'_def p''_def add_liquidity_spec_def add_liquidity_code_spec_def Let_def
     by (auto; metis add_divide_distrib eq_divide_eq_1 nonzero_eq_divide_eq order_less_irrefl)
   show "y p < y p'"
     by (simp add: add_liquidity_spec_def assms(1,2,4) l1 p'_def)
   show "y p' < y p''"
-    by (simp add: add_liquidity_code_def add_liquidity_spec_def l1 p''_def p'_def)
+    by (simp add: add_liquidity_code_spec_def add_liquidity_spec_def l1 p''_def p'_def)
   show "y p'' \<le> y p' + 1"
-    by (simp add: add_liquidity_code_def add_liquidity_spec_def l1 p''_def p'_def)
+    by (simp add: add_liquidity_code_spec_def add_liquidity_spec_def l1 p''_def p'_def)
   show "l p' - 1 < l p''"
-    by (simp add: add_liquidity_code_def add_liquidity_spec_def l1 p''_def p'_def) 
+    by (simp add: add_liquidity_code_spec_def add_liquidity_spec_def l1 p''_def p'_def) 
   show "l p'' \<le> l p'"
-    by (simp add: add_liquidity_code_def add_liquidity_spec_def l1 p''_def p'_def)
+    by (simp add: add_liquidity_code_spec_def add_liquidity_spec_def l1 p''_def p'_def)
+  show "l p \<le> l p''"
+    by (smt (z3) \<open>l p' - 1 < l p''\<close> add_liquidity_code_spec_def add_liquidity_spec_def assms(1) assms(3) assms(4) divide_less_eq_1_pos divide_pos_pos int_less_real_le nonzero_mult_div_cancel_right of_int_0 p''_def p'_def select_convs(3))
+  show "l p < l p'"
+    by (simp add: add_liquidity_spec_def assms(1) assms(3) assms(4) l1 p'_def)
   show "k p < k p'"
     by (simp add: \<open>x p < x p'\<close> \<open>y p < y p'\<close> assms(1,2) k_def less_eq_real_def mult_le_less_imp_less)
   show "k p' < k p''"
     by (metis \<open>x p < x p'\<close> \<open>x p' = x p''\<close> \<open>y p' < y p''\<close> assms(1) dual_order.strict_trans k_def mult.commute mult_less_iff1) 
-  show "(k p')/(k p) = ((l p')/(l p))^2"
+  show "k p'/k p = (l p'/l p)\<^sup>2"
     using assms(1-4) unfolding p'_def add_liquidity_spec_def Let_def k_def
     by (simp; algebra)
-  show "((l p'')/(l p))^2 < (k p'')/(k p)"
+  show "(l p''/l p)\<^sup>2 < k p''/k p"
   proof -
     have "((l p + \<lfloor>\<Delta>x * l p / x p\<rfloor>) / l p)\<^sup>2 \<le> ((l p + \<Delta>x * l p / x p) / l p)\<^sup>2"
     proof -
@@ -77,8 +84,185 @@ proof -
       by (smt (verit, ccfv_SIG) assms(1,2,4) less_divide_eq_1_pos linordered_comm_semiring_strict_class.comm_mult_strict_left_mono mult_less_cancel_right real_of_int_floor_add_one_gt times_divide_eq_left zero_less_mult_iff)
     ultimately
     show ?thesis
-      by (smt (verit, best) \<open>k p' / k p = (l p' / l p)\<^sup>2\<close> \<open>k p' < k p''\<close> add_liquidity_code_def add_liquidity_spec_def assms(1,2) divide_le_cancel k_def l1 p''_def p'_def select_convs(3) split_mult_pos_le)
+      by (smt (verit, best) \<open>k p' / k p = (l p' / l p)\<^sup>2\<close> \<open>k p' < k p''\<close> add_liquidity_code_spec_def add_liquidity_spec_def assms(1,2) divide_le_cancel k_def l1 p''_def p'_def select_convs(3) split_mult_pos_le)
   qed
+  show "x p / l p = x p' / l p'"
+    by (smt (verit) add_liquidity_spec_def assms(1) assms(4) divide_divide_eq_left divide_pos_pos nonzero_mult_div_cancel_left p'_def select_convs(1) select_convs(3))
+  show "y p / l p = y p' / l p'"
+    by (smt (verit, ccfv_SIG) add_liquidity_spec_def assms(1) assms(4) divide_nonneg_nonneg mult_divide_mult_cancel_left_if p'_def select_convs(2) select_convs(3))
+qed
+
+(*
+subsection "Implementation"
+
+record pool_state_impl =
+  x\<^sub>i :: machine_word
+  y\<^sub>i :: machine_word
+  l\<^sub>i :: machine_word
+
+definition add_liquidity_impl where
+  \<comment> \<open>TODO: deal with overflows\<close>
+  "add_liquidity_impl p \<Delta>x \<equiv>
+    \<lparr>x\<^sub>i = (x\<^sub>i p)+\<Delta>x,
+     y\<^sub>i = (y\<^sub>i p)+(((y\<^sub>i p)*\<Delta>x) div (x\<^sub>i p)),
+     l\<^sub>i = (l\<^sub>i p)+(((l\<^sub>i p)*\<Delta>x) div (x\<^sub>i p))\<rparr>"
+
+text \<open>
+  One idea is to do a*b/c it like this: https://stackoverflow.com/a/5542161.
+  Note that we'll need to adjust for the loss of precision that doing multiple divisions causes.
+  TODO: Prove that it works. Maybe first try it in cryptol.
+\<close>
+*)
+
+section "Removing liquidity"
+
+definition remove_liquidity_spec where
+  "remove_liquidity_spec p \<Delta>l \<equiv> let \<alpha> = \<Delta>l / l p
+    in \<lparr>x = (1-\<alpha>)*(x p), y = (1-\<alpha>)*(y p), l = (1-\<alpha>)*(l p)\<rparr>"
+
+definition remove_liquidity_code_spec where
+  "remove_liquidity_code_spec p \<Delta>l \<equiv>
+    \<lparr>x = x p - \<lfloor>\<Delta>l*(x p) / l p\<rfloor>,
+     y = y p - \<lfloor>\<Delta>l*(y p) / l p\<rfloor>,
+     l = l p - \<Delta>l\<rparr>"
+
+lemma l2:"(1 - \<Delta>l / l p) * a = a - \<Delta>l * a / l p" for a
+    \<comment> \<open>this simple lemma helps automated provers a lot\<close>
+  by algebra
+
+lemma remove_liquidity_properties:  
+  \<comment> \<open>properties of remove_liquidity\<close>
+  fixes p \<Delta>l
+  assumes "x p > 0" and "y p > 0" and "l p > 0"
+    and "\<Delta>l < l p" and "0 < \<Delta>l"
+  defines "p' \<equiv> remove_liquidity_spec p \<Delta>l"
+    and "p'' \<equiv> remove_liquidity_code_spec p \<Delta>l"
+  shows "x p' < x p" and "x p' \<le> x p''"
+    and "y p' < y p" and "y p' \<le> y p''"
+    and "l p' = l p''" and "l p' < l p"
+    and "k p' \<le> k p''" and "k p' < k p"
+    and "k p'/k p = (l p'/l p)\<^sup>2"
+    and "(l p''/l p)\<^sup>2 \<le> k p''/k p"
+    and "x p / l p = x p' / l p'"
+    and "y p / l p = y p' / l p'"
+proof -
+  show "x p' < x p"
+    by (smt (verit, del_insts) assms(1) assms(3) assms(5) divide_pos_pos l2 mult_pos_pos p'_def pool_state_spec.select_convs(1) remove_liquidity_spec_def)
+  show "x p' \<le> x p''"
+    by (simp add: assms(7) l2 p'_def remove_liquidity_code_spec_def remove_liquidity_spec_def)
+  show "y p' < y p"
+    by (smt (verit, best) assms(2) assms(3) assms(5) divide_pos_pos l2 mult_pos_pos p'_def pool_state_spec.select_convs(2) remove_liquidity_spec_def)
+  show "y p' \<le> y p''"
+    by (simp add: l2 p''_def p'_def remove_liquidity_code_spec_def remove_liquidity_spec_def)
+  show "l p' = l p''"
+    by (metis assms(3) l2 nonzero_mult_div_cancel_right not_less_iff_gr_or_eq p''_def p'_def pool_state_spec.select_convs(3) remove_liquidity_code_spec_def remove_liquidity_spec_def)
+  show "l p' < l p"
+    by (simp add: \<open>l p' = l p''\<close> assms(5) p''_def remove_liquidity_code_spec_def)
+  show "k p' < k p"
+    by (smt (verit) \<open>x p' < x p\<close> \<open>y p' < y p\<close> assms(1) assms(2) assms(3) assms(4) divide_less_eq_1_pos k_def mult_le_less_imp_less p'_def pool_state_spec.select_convs(2) remove_liquidity_spec_def zero_less_mult_iff)
+  show "k p' \<le> k p''"
+    by (smt (verit) \<open>x p' \<le> x p''\<close> \<open>y p' \<le> y p''\<close> assms(1) assms(2) assms(3) assms(4) divide_less_eq_1_pos k_def mult.commute mult_less_cancel_left_pos mult_pos_pos p'_def pool_state_spec.select_convs(1) pool_state_spec.select_convs(2) remove_liquidity_spec_def)
+  show "k p'/k p = (l p'/l p)\<^sup>2"
+    by (smt (verit, best) \<open>x p' < x p\<close> \<open>y p' < y p\<close> assms(3) k_def mult_cancel_right2 mult_divide_mult_cancel_left_if nonzero_eq_divide_eq nonzero_mult_div_cancel_left p'_def power2_eq_square remove_liquidity_spec_def select_convs(1) select_convs(2) select_convs(3) times_divide_eq_left)
+  show "(l p''/l p)\<^sup>2 \<le> k p''/k p"
+    by (metis \<open>k p' / k p = (l p' / l p)\<^sup>2\<close> \<open>k p' \<le> k p''\<close> \<open>l p' = l p''\<close> assms(1) assms(2) divide_right_mono k_def less_le_not_le split_mult_pos_le)
+  show "x p / l p = x p' / l p'"
+    by (smt (verit) assms(4) divide_divide_eq_right eq_divide_eq_1 mult.commute nonzero_mult_div_cancel_left p'_def remove_liquidity_spec_def select_convs(1) select_convs(3))
+  show "y p / l p = y p' / l p'"
+    by (smt (verit, best) \<open>x p / l p = x p' / l p'\<close> assms(1) divide_divide_eq_left divide_eq_0_iff nonzero_mult_div_cancel_left p'_def remove_liquidity_spec_def select_convs(2) select_convs(3))
+qed
+
+section "No free money"
+
+text \<open>Here we want to prove that, no matter what sequence of operations one applies,
+withdrawing all the liquidity obtained leaves the pool with at least the same amount of tokens it started from.
+We could formalize executions as lists, inductive invariants, etc.\<close>
+
+definition inv where
+  "inv p\<^sub>0 p \<equiv> l p > l p\<^sub>0 \<and> (
+    let p' = remove_liquidity_spec p (l p - l p\<^sub>0)
+    in x p' = x p\<^sub>0 \<and> y p' = y p\<^sub>0)"
+
+definition pool_nz where
+  "pool_nz p \<equiv> x p > 0 \<and> y p > 0 \<and> l p > 0"
+
+lemma l3:
+  fixes x l x' l' :: real
+  assumes "x/l = x'/l'" and "l>0" and "x>0"
+  shows "x'*(1-(l'-l)/l') = x"
+  by (metis (no_types, opaque_lifting) add.right_neutral add_diff_cancel assms diff_diff_eq diff_divide_distrib divide_divide_eq_right divide_eq_0_iff eq_divide_eq_1 minus_diff_eq mult_1 nonzero_eq_divide_eq order_less_irrefl times_divide_eq_left)   
+
+lemma l4:
+  fixes p\<^sub>0 p
+  assumes "inv p\<^sub>0 p" and "pool_nz p\<^sub>0" and "pool_nz p" and "l p \<ge> l p\<^sub>0"
+  shows "x p / l p = x p\<^sub>0 / l p\<^sub>0" and "y p / l p = y p\<^sub>0 / l p\<^sub>0"
+proof -
+  define p' where "p' \<equiv> remove_liquidity_spec p (l p - l p\<^sub>0)"
+  have 1:"l p\<^sub>0 = l p'"
+  proof -
+    have "(1 - (x' - x)/x')*x' = x" if "x' \<noteq> 0" for x x' :: real
+      by (simp add: diff_divide_distrib that)
+    thus ?thesis
+      unfolding p'_def remove_liquidity_spec_def Let_def
+      by (metis assms(3) order_less_irrefl pool_nz_def select_convs(3))
+  qed
+  have 2:"l p - l p\<^sub>0 > 0"
+    using AMM.inv_def assms(1) diff_gt_0_iff_gt by blast
+  have 3:"l p - l p\<^sub>0 < l p"
+    using assms(2) pool_nz_def by fastforce
+  show "x p / l p = x p\<^sub>0 / l p\<^sub>0"
+  proof -
+    have "x p / l p = x p' / l p'"
+      using "2" "3" assms(3) p'_def pool_nz_def remove_liquidity_properties(11) by blast
+    thus ?thesis using 1
+      by (metis AMM.inv_def assms(1) p'_def)
+  qed
+  show "y p / l p = y p\<^sub>0 / l p\<^sub>0"
+  proof -
+    have "y p / l p = y p' / l p'"
+      using "2" "3" assms(3) p'_def pool_nz_def remove_liquidity_properties(12) by blast
+    thus ?thesis using 1
+      by (metis AMM.inv_def assms(1) p'_def)
+  qed
+qed
+
+lemma l5:
+  fixes p\<^sub>0 p p' \<Delta>x
+  assumes "inv p\<^sub>0 p" and "l p' \<ge> l p" and "l p \<ge> l p\<^sub>0" and "pool_nz p\<^sub>0" and "pool_nz p"
+    and "x p' / l p' = x p / l p" and "y p' / l p' = y p / l p"
+  shows "inv p\<^sub>0 p'"
+proof -
+  define p'' where "p'' \<equiv> remove_liquidity_spec p' (l p' - l p\<^sub>0)"
+  have "x p\<^sub>0 / l p\<^sub>0 =  x p' / l p'"
+    by (metis assms(1) assms(3) assms(4) assms(5) assms(6) l4(1))
+  hence "x p\<^sub>0 = x p''" using l3 unfolding p''_def remove_liquidity_spec_def Let_def
+    by (metis assms(4) mult.commute pool_nz_def select_convs(1))
+  have "y p\<^sub>0 / l p\<^sub>0 =  y p' / l p'"
+    using assms(1) assms(3) assms(4) assms(5) assms(7) l4(2) by fastforce
+  hence "y p\<^sub>0 = y p''" using l3 unfolding p''_def remove_liquidity_spec_def Let_def
+    by (metis assms(4) mult.commute pool_nz_def select_convs(2))
+  show ?thesis
+    by (metis AMM.inv_def \<open>x p\<^sub>0 = x p''\<close> \<open>y p\<^sub>0 = y p''\<close> assms(1) assms(2) dual_order.strict_trans1 p''_def)
+qed
+
+lemma inv_add_okay:
+  fixes p\<^sub>0 p p' \<Delta>x
+  assumes "inv p\<^sub>0 p" and "0 < \<Delta>x" and "pool_nz p\<^sub>0" and "pool_nz p"
+  defines "p' \<equiv> add_liquidity_spec p \<Delta>x"
+  shows "inv p\<^sub>0 p'"
+proof -
+  have "x p' / l p' = x p / l p" and "y p' / l p' = y p / l p"
+     apply (metis add_liquidity_properties(14) assms(2) assms(4) p'_def pool_nz_def)
+    apply (metis add_liquidity_properties(15) assms(2) assms(4) p'_def pool_nz_def)
+    done
+  moreover
+  have "l p' \<ge> l p"
+    using add_liquidity_properties(9) assms(2) assms(4) less_le_not_le p'_def pool_nz_def by blast
+  moreover
+  have "l p \<ge> l p\<^sub>0"
+    using AMM.inv_def assms(1) less_le_not_le by blast
+  ultimately show ?thesis using l5
+    using assms(1) assms(3) assms(4) by blast
 qed
 
 end
